osiris/test/sample_record.ml
@@ -1,0 +1,6 @@
+type t = { rx : int; ry : int }
+
+let r1 = { rx = 1; ry = 2 }
+let r2 = { ry = 4; rx = 3 }
+let get_y r = r.ry
+let set_x r = { r with rx = 5 }
